---
layout: post
title: Math 6302 Pset 4
last_updated: 2025-05-11
---

[comment]: THIS FILE IS AUTOMATICALLY GENERATED FROM Math6302Pset4.tex. IT WILL BE REWRITTEN ON CHANGE OF THE .tex FILE!

> **Problem:**
>
> > **Subproblem:**
> >
> > To begin we show addition
> > $$\sigma_k(r_1+r_2) = (r_1+r_2)(e^{(2k-1)\pi i/n} = r_1e^{(2k-1)\pi i/n} + r_2 e^{(2k-1)\pi i/n} = \sigma_k(r_1)+\sigma_k(r_2)$$
> > And also that multiplication holds
> > $$\sigma_k(r_1r_2) = (r_1r_2)(e^{(2k-1)\pi i/n}) = (r_1)(e^{(2k-1)\pi i/n})\cdot (r_2)(e^{(2k-1)\pi i/n}) = \sigma_k(r_1)\cdot \sigma_k(r_2)$$
> > Note that this works since $e^{(2k-1)\pi i/n}$ is a root of $x^n+1$
> > and since any multiple of $x^n+1$ evaluates to 0 we
> > multiplicativity.
> >
> > Now to show bijectivity,
> >
> > Suppose
> > $\exists r\in \mathbb{Z}[x]/(x^n+1)\ \text{s.t.} \ \sigma_k(r)=0$
> > with $r(x)=r_0 + r_1 x +\cdots + r_{n-1}x^{n-1}$. Then
> > $\sigma_k(r) = r (e^{\pi i /n}) = 0$ but since if
> > $p(e^{\pi i/n}) = 0$ for a integer polynomial $p$, then $p$ is
> > divisible by $x^n+1$. Thus in $\mathbb{Z}[x]/(x^n+1)$,
> > $r(x)\equiv 0\mod x^n+1\Rightarrow r=0$. Thus since the kernel of
> > $\sigma_k$ is just 0 which implies injectivity.
> >
> > Now also since any element in $\mathbb{Z}[e^{\pi i/n}]$ can be
> > written as $$r_0 + r_1 e^{\pi i/n} + \cdots + r_m(e^{\pi i/n})^m$$
> > With $r_i\in \mathbb{Z}, m\in \mathbb{N}$. Thus since
> > $e^{\pi i n/n } = -1$ implies that every element in
> > $\mathbb{Z}[e^{\pi i /n}]$ can be expressed as a linear combination
> > of integer coefficents of the basis
> > $$1, e^{\pi i/n}, \cdots, (e^{\pi i/n})^{n-1}$$ Now let
> > $r(x)=r_0 + r_1x +\cdots + r_{n-1}x^{n-1}\in \mathbb{Z}[x]/(x^n+1)$
> > represented by $\sigma_k(x)=(e^{(2k-1)\pi i/n})^m$ such that
> > $(2k-1)m\equiv 1\mod 2n$. Thus
> > $$\sigma_k(r(x^m)) =r_0 + r_1 e^{\pi i /n} + \cdots + r_{n-1} (e^{\pi i/n})^{n-1}$$
> > Thus any element in $\mathbb{Z}[e^{\pi i/n}]$ is in the image of an
> > $r\in \mathbb{Z}[x]/(x^n+1)$ which implies surjectivity.
> >
> > Thus since we have shown bijectviity, additivity, and
> > multiplicativity which implies $\sigma_k$ is a ring isomorhism. 0◻
>
> > **Subproblem:**
> >
> > For any ring homomorphism that maps to $\mathbb{C}$
> > $$\sigma^*(0)=\sigma^*(x)^n+\sigma^*(1)$$ Thus this implies that
> > $\sigma^*(x)^n + 1 = 0$ since $\sigma^*(0)=0, \sigma^*(1)=1$ by
> > definition of a ring homomorphism.
> >
> > This implies that $\sigma^*$ is a root in $x^n+1=0$. Thus since
> > there is a bound of $n$ roots implies that there exists some
> > $k\in [n]$ such that $$\sigma^*(x)=e^{(2k-1)\pi i/n}$$ This implies
> > that for any element $r\in \mathbb{Z}[x]/(x^n+1)$ that
> > $$\sigma^*(r)=\sum_{i=0}^{n-1}r_i(\sigma^*(x))^i$$ and
> > $$\sigma_k(r)=\sum_{i=0}^{n-1}r_i(\sigma_k(x))^i$$ Finally since
> > $\sigma_k(r)=\sigma^*(r)$ then they are equivalent 0◻
>
> > **Subproblem:**
> >
> > Given $r\in \mathbb{Z}[x]/(x^n+1)$, then
> > $$||\sigma(r)||^2 = \sum_{k=1}^n |\sigma_k(r)|^2=\sum_{k=1}^n \sigma_k(r)\overline{\sigma_k(r)}$$
> > Now since $\sigma_k(r) = \sum_{i=0}^{n-1}r \omega_k^i$ and
> > $\overline{\sigma_k(r)} = \sum_{j=0}^{n-1}r_j w_k^{-j}$ Then
> > $$||\sigma(r)||^2 = \sum_{k=1}^n (\sum_{i=0}^{n-1}r_i \omega_k^i)(\sum_{j=0}^{n-1}r_j\omega_k^{-j}) = \sum_{i,j=0}^{n-1}r_ir_j \sum_{k=1}^n \omega_k^{i-j}$$
> > But since $\omega_k = e^{(2k-1)\pi i/n}$ implies that there are $2n$
> > roots of unity where $\omega_k^n=-1$. This implies that
> > $\sum_{k=1}^n \omega_k^m$ is equal to $n$ if $m\equiv 0\mod n$ and 0
> > otherwise. Thus we can simplity our equation to be
> > $$\sum_{i,j=0}^{n-1}r_ir_j \sum_{k=1}^n \omega_k^{i-j} = n\sum_{i=0}^{n-1}r_i^2 = n||r||^2$$
> > and thus square rooting each side implies that
> > $$||\sigma_k(r)|| = \sqrt{n}||r||$$0◻
>
> > **Subproblem:**
> >
> > Let $S=\sigma(r)$ for each
> > $r\in \mathbb{Z}[x]/(x^n+1)) \subset \mathbb{C}^n$. Then for any
> > $\sigma(r_1), \sigma(r_2)\in S$,
> > $$\sigma(r_1)+\sigma(r_2)=(\sigma_1(r_1)+\sigma_2(r_2), \cdots, \sigma_n(r_1)+ \sigma_n(r_2))$$
> > And since $\sigma_k$ is a ring homomorphism implies
> > $$=\sigma(r_1+r_2)$$
> >
> > Similarly,
> > $$\sigma(r_1)\sigma(r_2)=(\sigma_1(r_1)\sigma_2(r_2), \cdots, \sigma_n(r_1) \sigma_n(r_2))$$
> > And since $\sigma_k$ is a ring homomorphism implies
> > $$=\sigma(r_1r_2)$$
> >
> > Now suppose there is a $r_1 r_2 = 0$. Then since $\mathbb{C}$ has no
> > zero divisors, $\forall k$, $\sigma_k(r_1)=0$ or $\sigma_k(r_2)=0$.
> > But due to the fact that $\sigma_k$ is injective in 1.1 so then
> > $\sigma_k(r)=0\Rightarrow r=0$. Thus $S$ has no nontrivial zero
> > divisors.
> >
> > Define a map between the two as $z\in \sqrt{n}\mathbb{Z}^n$ as
> > $$A:z\mapsto (\sigma_1(z\frac{1}{\sqrt{n}}), \cdots, \sigma_n(z\frac{1}{\sqrt{n}}))$$
> > Then this map is linear since we showed that $\sigma_k$ is linear by
> > definition. We also know this map is length preserving since
> > $$(\sigma_1(z\frac{1}{\sqrt{n}}), \cdots, \sigma_n(z\frac{1}{\sqrt{n}})) = ||\sigma(z\frac{1}{\sqrt{n}})|| = \sqrt{n} ||z\frac{1}{\sqrt{n}}||= ||z||$$

> **Problem:**
>
> > **Subproblem:**
> >
> > We claim that the explicit generator for $s$ that makes
> > $\mathcal{I}$ ideal is $s=1$. Now let $r_1=x, r_2=-3x-2$. Then
> > $$5r_1+r_2(1+x) 5x + (-3x-2)(1+x) = 5x -3x-3x^2-2-2x = -2-3x^2$$ But
> > since we are working in $\mathbb{Z}[x]/(x^2+1)$ implies that
> > $x^n=-1, n=2$ so $-2-3x^2 = 3-2 =1 = s$. Thus $s\in \mathcal{I}$.
> > Now let $r_1=1=s, r_2 = 0$. Thus $5\cdot1 + 0(1+x) = 5$ Now let
> > $r_1=0,r_2=1=s$. Thus $5\cdot0+1(1+x) = 1+x$. Thus we have shown
> > $x+1$ and $5$ are contianed in the ieal generated by $s$. Thus we
> > have shown both properties and $\mathcal{I}$ is a principal ideal
> > with explicit generator $s=1$.0◻
>
> > **Subproblem:**
> >
> > Assume that it is a principle ideal. Then
> > $\mathcal{I} = \{2r_1 + r_2(1+x)\}, r_1,r_2\in R$. Then if it is
> > principle there exists $s\in R$ such that $s = a+bx$,
> > $a,b\in \mathbb{Z}$. So then if $I=(s)$, $s$ divides every element
> > inthe ideal. This implies that $s$ divides $2, 1+x$.
> >
> > Now using multiplictive norms, let
> > $$N:R\to \mathbb{Z}, N(a+bx)=a^2 3b^2$$
> >
> > Then the norms of the divisibility relations are
> > $$N(s)|N(2)=4, N(s)|N(1+x)=4$$ So $N(s)\in \{1,2,4\}$.
> >
> > Now since $N(s)=2$ is impossible since $a^2+3b^2\equiv 0,1 p\mod 3$
> >
> > Now since $N(s)=4$ gives $b=0, |a|=2$ so $s\pm 2$ but if $s\pm 2$
> > then $\pm2|(1+x)$ implies $(1+x)/2 \in R$ which is not true. And if
> > $|a|=|b|=1$ then $s=\pm (1\pm x)$ and $2=sq$, $q$ being the quotient
> > so $N(s)N(q) = 4 = 4N(q)$ so $N(q)=1,q=\pm 1$. Thus $N(s)\neq 4$.
> >
> > This means that $N(s)$ must be $1$ which implies that $s=\pm 1$.
> > This would imply that any common divisor of 2 and $1+x$ is a unit.
> >
> > Now suppose $1\in \mathcal{I}$. Then
> > $\exists r_1,r_2\in R \ \text{s.t.} \ 1=2r_1+r_2(1+x)$. But since
> > every element of $R=\mathbb{Z}[x]/(x^2+3)$ can be uniquely wirtten
> > as $a+bx$, $a,b\in \mathbb{Z}$ then let $r_1=a+bx, r_2 = c+dx$
> > implies that $$1 = 2a+2bx+c+dx+cx+dx^2$$ So then since $x^2=-3$ in
> > $R$, $dx^2=-3d$. Thus $$1 = (2a+c-2d) + x(2b+c+d)$$ This gives a
> > system of two equations $$1=2a+c-3d$$ $$2b+c+d=0$$ And since they
> > have the same partiy both of these equations cannot satisfy, hence a
> > contradiction. and $1\notin \mathcal{I}$.
> >
> > Now since we showed that if $I=(s)$ was principal that its generator
> > is a common divisor of $2$ and $1+x$ so $s=\pm1$ and $\mathcal{I}=R$
> > but $\mathcal{I}!=R$ so we have a contradiction. Thus it is not a
> > principle ideal.0◻
>
> > **Subproblem:**
> >
> > Now since if $n$ is a power of two the polynomial $x^n+1$ becomes
> > irreducible implies that there are no factors over $\mathbb{Z}$.
> > This then implies that the quotient ring $R = \mathbb{Z}[x]/(x^n+1)$
> > does not contian a zero divisor.
> >
> > Now since $s_1R = s_2R$ implies that $s_1$ divides $s_2$
> > $s_2 = us_1$ and that $s_2$ divides $s_1$ $s_1 = vs_2$. This implies
> > that $s_1 = v(us_1) = (vu)s_1$ by associativity. Thus $s_1(1-vu)=0$.
> > But since since the integral domain does not contain a zero divisor
> > and $s_1\neq 0$ then $1-vu=0\Rightarrow vu =1$ which implies that
> > $v=u^{-1}$ and $u^{-1}u=1$.0◻

> **Problem:**
>
> > **Subproblem:**
> >
> > Recall that a hexagonal lattice can be represented with a basis of
> > $$\begin{bmatrix}1&-\frac 12\\0&\sqrt 3 /2 \end{bmatrix}$$ Then
> > $||b_1|| = 1 = \lambda_1(\mathcal{L})$ and so
> > $\Pi_2(b_2) = \begin{bmatrix}0\\\frac{\sqrt 3}{2}\end{bmatrix}$
> > which is the shortest vector in $\Pi_2(\mathcal{L})$. Thus it is a
> > HKZ reduced basis. So doing ghram schmidt on it we trivially get
> > that
> > $||\tilde{b}_1|| = \lvert  \rvert\begin{bmatrix}1\\0\end{bmatrix}|| = 1$
> > and then
> > $$||\tilde{b_2}|| = ||\Pi_{b_1^\perp}(b_2)|| = \lvert  \rvert\begin{bmatrix}0\\ \frac{\sqrt 3}{2}\end{bmatrix}|| = \frac{\sqrt3}{2}$$
> > So then
> > $$\frac{||\tilde{b}_1||}{||\tilde{b}_2||} = \frac1{\sqrt3/2} = \frac2{\sqrt3}$$
>
> > **Subproblem:**
> >
> > Recall that minkowskis theorem states
> > $$\lambda_1(\mathcal{L}) \leq \sqrt{\gamma_j}\mathrm{vol}(L)^{\frac1j}$$
> > Now given $j$, consider the $j$ dimensional sublattice
> > $\mathcal{L}' = \Pi_{n-k+1}(\mathcal{L})$. Thus
> > $$\mathrm{vol}(L')=\Pi_{k=1}^j \lvert  \rvert\tilde{b}_{n-j+k}||$$
> > and $\lambda_1(\mathcal{L}') = ||\tilde{b}_{n-j+1}||$ by the
> > definition of a HKZ reduced basis. We also know that
> > $\gamma_j\leq j\forall j$. This implies that
> > $$||\tilde{b}_{n-j+1}||\leq \sqrt{j}(\Pi_{k=1}^j||\tilde{b}_{n-j+k}||)^{\frac1j}$$
> > So raising everying by $j$, diving by $||\tilde{b}_{n-j+1}||$, and
> > rearranging indices implies that
> > $$||\tilde{b}_{n-j+1}||^{j-1}\leq j^{j/2} \Pi_{k=1}^{j-1} ||\tilde{b}_{n-k+1}||$$
> > Thus this implies that
> > $$||\tilde{b}_{n-j+1}||\leq j^{j/(2(j-1))} \Pi_{k=1}^{j-1} ||\tilde{b}_{n-k+1}||^{1/(j-1)}$$
> > And so squaring everyhing implies that
> > $$||\tilde{b}_{n-j+1}||^2\leq j^{j/(j-1)} \Pi_{k=1}^{j-1} ||\tilde{b}_{n-k+1}^{2/(j-1)}$$0◻
>
> > **Subproblem:**
> >
> > To begin, lets prove the base case of $j=2$.
> > $$||\tilde{b}_{n-2+1}||^2 \leq 2^{2/1} \Pi_{k=1}^{1}$$
> > $$||\tilde{b}_{n-k+1}||^2\Rightarrow ||\tilde{b}_{n-1}||^2 \leq 4 ||\tilde{b}_{n}||^2$$
> > And since Question 3.1 implies that
> > $\frac{||\tilde{b}_n||}{||\tilde{b}_{n-1}||} = \sqrt3/2 \leq 2 \leq \sqrt4$
> > implies that this is true. Thus the $j=2$ base case holds. Now to
> > induct over $j$. Suppose this holds at $j$. Then to induct over $j$
> > assume
> > $$||\tilde{b}_{n-j+1}||^2 \leq j (\Pi_{k=2}^j k^{1/(k-1)}) ||\tilde{b}_n||^2$$
> > is true. Then by equation 1
> > $$||\tilde{b}_{n-j}|| \leq (j+1)^{(j+1) /j} \Pi_{k=1}^j ||\tilde{b}_{n-k+1}||^{2/(j)}$$
> > $$= (j+1)^{1+1/j} ( \|\tilde{b}_{n-j+1}\|^{2/j} \prod_{i=1}^{j-1} \|\tilde{b}_{n-i+1}\|^{2/j} )$$
> > So by applying the inductive hypothesis to each term we get
> > $$\leq (j+1)^{1+1/j} ( \left( j \prod_{k=2}^j k^{1/(k-1)} \|\tilde{b}_n\|^2 \right)^{2/j} \prod_{i=1}^{j-1} \left( (j-i+1) \prod_{k=2}^{j-i+1} k^{1/(k-1)} \|\tilde{b}_n\|^2 \right)^{2/j} )$$
> > Which implies that by simplyfing evaluating the nested
> > $\Pi_{k=2}^r k^{1/(k-1)}$ terms and applying an exponent of $2/j$
> > with rearranging we get
> > $$= (j+1) \left( \prod_{k=2}^{j+1} k^{1/(k-1)} \right) \|\tilde{b}_n\|^2$$
> > Thus by mathematical induction this holds 0◻
>
> > **Subproblem:**
> >
> > Recall that since
> > $$||\tilde{b}_{n-j+1}||^2\leq j \cdot (\Pi_{k=2}^j k^{1/(k-1)})\cdot ||\tilde{b}_n||^2 \Rightarrow$$
> > $$\frac{||\tilde{b}_{n-j+1}||^2}{||\tilde{b}_n||^2}\leq j \cdot (\Pi_{k=2}^j k^{1/(k-1)})$$
> > Now since $2\leq k\leq j\leq n$ since $k$ is always greater than 1
> > and its exponent is greater than 0 we know that
> > $k^{1/(k-1)} \leq n^{1/(k-1)}\forall 2\leq k\leq n$. Thus
> > $$j \cdot (\Pi_{k=2}^j k^{1/(k-1)}) \leq j\cdot(\Pi_{k=2}^j n^{1/(k-1)}) \leq n \cdot (\Pi_{k=2}^j n^{1/(k-1)}) = n\cdot (n^{\sum_{k=2}^j 1/(k-1)})$$
> > And using the fact about harmonic numbers
> > $H_n := \sum_{i=1}^n 1/i \Rightarrow H_n \leq \log(n)+1$ imples that
> > $$n\cdot (n^{\sum_{k=2}^j 1/(k-1)})\leq n\cdot(n^{\log(j)+1})$$ And
> > since we know that $\log(j)\leq \log(n) \forall 2\leq j \leq n,$
> > $$n\cdot(n^{\log(j)+1}) \leq n\cdot(n^{\log(n)+1}) = n^{\log(n)+2}$$
> > Thus we have shown that
> > $$\frac{||\tilde{b}_{n-j+1}||^2}{||\tilde{b_n}||^2}\leq n^{\log(n)+2}$$
> > Now since we have shown it for any possible $j$ implies that
> > $$\max_{1\leq j\leq n}\frac{||\tilde{b}_{n-j+1}||^2}{||\tilde{b_n}||^2}\leq n^{\log(n)+2}$$
>
> > **Subproblem:**
> >
> > Given $(b_1,\cdots,b_i)4$, $||b_1||$ is still equal to
> > $\lambda_1(\mathcal{L})$. Similarly, for any
> > $k \in \{1,\cdots i\}, (\Pi_k(b_k), \cdots, \Pi_k(b_i))$ is still an
> > HKZ reduced basis since $(\Pi_k(b_k)),\cdots, \Pi_k(b_n))$ is a HKZ
> > reduced basis.
> >
> > Thus both axioms of a HKZ reduced basis still satisfy.
> >
> > Now given
> > $$\omega(B) = \max_{j\geq i}\frac{||\tilde{b}_i||}{||\tilde{b}_j||}$$
> > Implies that since
> > $$\max_{1\leq j\leq n}\frac{||\tilde{b}_{n-j+1}||^2}{||\tilde{b_n}||^2}\leq n^{\log(n)+2}$$
> > That $\omega(B) \leq \sqrt{n^{\log(n)+2}} = n^{\log(n)/2 + 1}$ 0◻

> **Problem:**
>
> A like 20 hours
